common/theories/LoopChecking/Interfaces.v
@@ -2,7 +2,7 @@
 From Stdlib Require Import ssreflect ssrbool ZArith.
 From Stdlib Require Import Program RelationClasses Morphisms.
 From Stdlib Require Import Orders OrderedTypeAlt OrderedTypeEx MSetList MSetInterface MSetAVL MSetFacts FMapInterface MSetProperties MSetDecide.
-From MetaRocq.Utils Require Import utils.
+From MetaRocq.Utils Require Import utils NonEmptyLevelExprSet.
 
 From MetaRocq.Common Require Universes.
 From MetaRocq.Common Require Import LoopChecking.Common.
@@ -44,27 +44,29 @@ Module Type FMapOTInterface (E : UsualOrderedType).
   Include FMapInterface.Sfun OT.
 End FMapOTInterface.
 
+Module Q <: Quantity.
+  Include OrdersEx.Z_as_OT.
+  Definition reflect_eq : ReflectEq t := _.
+  Definition eq_leibniz x y : eq x y -> x = y := fun e => e.
+End Q.
+
 Module Type LevelSets.
   (* Signature of levels: decidable, ordered type *)
-  Declare Module Level : LevelOrderedTypeWithReflect.
+  Declare Module Level : OrderedTypeWithLeibnizWithReflect.
   Declare Module LevelSet : LevelSet_fun Level.
-  Declare Module LevelExpr : LevelExprItf Level.
-  Declare Module LevelExprSet : LevelExprSet_fun Level LevelExpr.
+  Declare Module LevelExpr : LevelExprT Level Q.
+  Declare Module LevelExprSet : LevelExprSet_fun Level Q LevelExpr.
   Declare Module LevelMap : FMapOTInterface Level.
 End LevelSets.
 
 Module FromLevelSets (LS : LevelSets).
 Export LS.
 
-Definition level (e : LevelExpr.t) : Level.t := fst e.
-Coercion level : LevelExpr.t >-> Level.t.
-Extraction Inline level.
+Module NES := NonEmptyLevelExprSet Level Q LevelSet LevelExpr LevelExprSet.
+Import NES.
 
-Definition levels (e : LevelExprSet.t) :=
-LevelExprSet.fold (fun le => LevelSet.add (level le)) e LevelSet.empty.
-Export LevelExprSet (nonEmptyLevelExprSet, t_set, t_ne).
-
-Existing Instance Level.reflect_eq.
+#[export] Existing Instance Level.reflect_eq.
+#[export] Existing Instance NES.reflect_eq.
 
 Module LevelSetFact := WFactsOn Level LevelSet.
 Module LevelSetProp := WPropertiesOn Level LevelSet.
@@ -95,36 +97,10 @@ Definition print_lset (l : LevelSet.t) :=
 Module LevelExprSetFact := WFactsOn LevelExpr LevelExprSet.
 Module LevelExprSetProp := WPropertiesOn LevelExpr LevelExprSet.
 
-(* We have decidable equality w.r.t leibniz equality for sets of levels. *)
-#[global, program] Instance levelexprset_reflect : ReflectEq LevelExprSet.t :=
-  { eqb := LevelExprSet.equal }.
-Next Obligation.
-  destruct (LevelExprSet.equal x y) eqn:e; constructor.
-  eapply LevelExprSet.equal_spec in e.
-  now eapply LevelExprSet.eq_leibniz.
-  intros e'.
-  subst y.
-  pose proof (@LevelExprSetFact.equal_1 x x).
-  forward H. reflexivity. congruence.
-Qed.
-
 #[global] Instance levelexprset_eq_dec : Classes.EqDec LevelExprSet.t := Classes.eq_dec.
 
-Derive NoConfusion for LevelExprSet.nonEmptyLevelExprSet.
+Derive NoConfusion for NES.t.
 
-(* We use uip on the is_empty condition *)
-#[global, program] Instance nonEmptyLevelExprSet_reflect : ReflectEq nonEmptyLevelExprSet :=
-  { eqb x y := eqb x.(t_set) y.(t_set) }.
-Next Obligation.
-  destruct (eqb_spec (t_set x) (t_set y)); constructor.
-  destruct x, y; cbn in *. subst.
-  now rewrite (uip t_ne0 t_ne1).
-  intros e; subst x; apply H.
-  reflexivity.
-Qed.
-
-(** This coercion allows to see the non-empty set as a regular [LevelExprSet.t] *)
-Coercion t_set : nonEmptyLevelExprSet >-> LevelExprSet.t.
 Module LevelExprSetDecide := WDecide (LevelExprSet).
 Ltac lesets := LevelExprSetDecide.fsetdec.
 
@@ -162,251 +138,6 @@ Proof.
   now eapply LevelSet.choose_spec1 in ch.
   now apply LevelSet.choose_spec2 in ch.
 Qed.
-
-Module NonEmptySetFacts.
-  #[program] Definition singleton (e : LevelExpr.t) : nonEmptyLevelExprSet
-    := {| t_set := LevelExprSet.singleton e |}.
-  Next Obligation.
-    apply negbTE.
-    eapply (contra_notN (P := LevelExprSet.Empty (LevelExprSet.singleton e))).
-    apply LevelExprSetFact.is_empty_2. intros ne. red in ne. specialize (ne e). lesets.
-  Qed.
-
-  Lemma not_Empty_is_empty s :
-    ~ LevelExprSet.Empty s <-> LevelExprSet.is_empty s = false.
-  Proof.
-    split.
-    - intro H. apply not_true_is_false. intro H'.
-      apply H. now apply LevelExprSetFact.is_empty_2 in H'.
-    - intros H he. red in he. apply negbT in H. unshelve eapply (contraNnot _ H).
-      3:exact he. intros ha. now apply LevelExprSetFact.is_empty_1.
-  Qed.
-
-  Program Definition add (e : LevelExpr.t) (u : nonEmptyLevelExprSet) : nonEmptyLevelExprSet
-    := {| t_set := LevelExprSet.add e u |}.
-  Next Obligation.
-    apply not_Empty_is_empty; intro H.
-    eapply H. eapply LevelExprSet.add_spec.
-    left; reflexivity.
-  Qed.
-
-  Lemma add_spec e u e' :
-    LevelExprSet.In e' (add e u) <-> e' = e \/ LevelExprSet.In e' u.
-  Proof.
-    apply LevelExprSet.add_spec.
-  Qed.
-
-  Definition add_list : list LevelExpr.t -> nonEmptyLevelExprSet -> nonEmptyLevelExprSet
-    := List.fold_left (fun u e => add e u).
-
-  Lemma add_list_spec l u e :
-    LevelExprSet.In e (add_list l u) <-> In e l \/ LevelExprSet.In e u.
-  Proof.
-    unfold add_list. rewrite <- fold_left_rev_right.
-    etransitivity. 2:{ eapply or_iff_compat_r. etransitivity.
-                        2: apply @InA_In_eq with (A:=LevelExpr.t).
-                        eapply InA_rev. }
-    induction (List.rev l); cbn.
-    - split. intuition. intros [H|H]; tas. invs H.
-    - split.
-      + intro H. apply add_spec in H. destruct H as [H|H].
-        * left. now constructor.
-        * apply IHl0 in H. destruct H as [H|H]; [left|now right].
-          now constructor 2.
-      + intros [H|H]. inv H.
-        * apply add_spec; now left.
-        * apply add_spec; right. apply IHl0. now left.
-        * apply add_spec; right. apply IHl0. now right.
-  Qed.
-
-  Lemma elements_not_empty {u : nonEmptyLevelExprSet} : LevelExprSet.elements u <> [].
-  Proof.
-    rewrite -LevelExprSetProp.elements_Empty.
-    move/LevelExprSetFact.is_empty_1.
-    destruct u as [u1 u2]; cbn in *. congruence.
-  Qed.
-
-  Equations to_nonempty_list (u : nonEmptyLevelExprSet) : LevelExpr.t * list LevelExpr.t :=
-  | u with inspect (LevelExprSet.elements u) := {
-    | exist [] eqel => False_rect _ (elements_not_empty eqel)
-    | exist (e :: l) _ => (e, l) }.
-
-  Lemma singleton_to_nonempty_list e : to_nonempty_list (singleton e) = (e, []).
-  Proof.
-    funelim (to_nonempty_list (singleton e)). bang.
-    clear H.
-    pose proof (LevelExprSet.singleton_spec e1 e).
-    rewrite LevelExprSetFact.elements_iff in H.
-    rewrite InA_In_eq in H. rewrite e0 in H.
-    destruct H. forward H. now left. noconf H. f_equal.
-    pose proof (LevelExprSet.cardinal_spec (LevelExprSet.singleton e1)). rewrite e0 in H. cbn in H.
-    rewrite LevelExprSetProp.singleton_cardinal in H.
-    destruct l => //.
-  Qed.
-
-  Lemma to_nonempty_list_spec u :
-    let '(e, u') := to_nonempty_list u in
-    e :: u' = LevelExprSet.elements u.
-  Proof.
-    funelim (to_nonempty_list u). bang. now rewrite e0.
-  Qed.
-
-  Lemma to_nonempty_list_spec' u :
-    (to_nonempty_list u).1 :: (to_nonempty_list u).2 = LevelExprSet.elements u.
-  Proof.
-    pose proof (to_nonempty_list_spec u).
-    now destruct (to_nonempty_list u).
-  Qed.
-
-  Lemma In_to_nonempty_list (u : nonEmptyLevelExprSet) (e : LevelExpr.t) :
-    LevelExprSet.In e u
-    <-> e = (to_nonempty_list u).1 \/ In e (to_nonempty_list u).2.
-  Proof.
-    etransitivity. symmetry. apply LevelExprSet.elements_spec1.
-    pose proof (to_nonempty_list_spec' u) as H.
-    destruct (to_nonempty_list u) as [e' l]; cbn in *.
-    rewrite <- H; clear. etransitivity. apply InA_cons.
-    eapply or_iff_compat_l. apply InA_In_eq.
-  Qed.
-
-  Lemma In_to_nonempty_list_rev (u : nonEmptyLevelExprSet) (e : LevelExpr.t) :
-    LevelExprSet.In e u
-    <-> e = (to_nonempty_list u).1 \/ In e (List.rev (to_nonempty_list u).2).
-  Proof.
-    etransitivity. eapply In_to_nonempty_list.
-    apply or_iff_compat_l. apply in_rev.
-  Qed.
-
-
-  Program Definition non_empty_union (u v : nonEmptyLevelExprSet) : nonEmptyLevelExprSet :=
-    {| t_set := LevelExprSet.union u v |}.
-  Next Obligation.
-    apply not_Empty_is_empty; intro H.
-    assert (HH: LevelExprSet.Empty u). {
-      intros x Hx. apply (H x).
-      eapply LevelExprSet.union_spec. now left. }
-    apply LevelExprSetFact.is_empty_1 in HH.
-    rewrite t_ne in HH; discriminate.
-  Qed.
-
-
-  Lemma eq_univ (u v : nonEmptyLevelExprSet) :
-    u = v :> LevelExprSet.t -> u = v.
-  Proof.
-    destruct u as [u1 u2], v as [v1 v2]; cbn. intros X; destruct X.
-    now rewrite (uip_bool _ _ u2 v2).
-  Qed.
-
-  Lemma eq_univ_equal (u v : nonEmptyLevelExprSet) :
-    LevelExprSet.Equal u v <-> u = v.
-  Proof.
-    split.
-    - intro H. now apply eq_univ, LevelExprSet.eq_leibniz.
-    - intros ->; reflexivity.
-  Qed.
-
-  Lemma eq_univ_elements (u v : nonEmptyLevelExprSet) :
-    LevelExprSet.elements u = LevelExprSet.elements v -> u = v.
-  Proof.
-    intro H. apply eq_univ.
-    destruct u as [u1 u2], v as [v1 v2]; cbn in *; clear u2 v2.
-    eapply LevelExprSet.eq_leibniz. red.
-    intros x. rewrite -!LevelExprSet.elements_spec1 H //.
-  Qed.
-
-  Lemma univ_expr_eqb_true_iff (u v : nonEmptyLevelExprSet) :
-    LevelExprSet.equal u v <-> u = v.
-  Proof.
-    split.
-    - intros.
-      apply eq_univ_equal. now apply LevelExprSet.equal_spec.
-    - intros ->. now apply LevelExprSet.equal_spec.
-  Qed.
-
-  Lemma univ_expr_eqb_comm (u v : nonEmptyLevelExprSet) :
-    LevelExprSet.equal u v <-> LevelExprSet.equal v u.
-  Proof.
-    transitivity (u = v). 2: transitivity (v = u).
-    - apply univ_expr_eqb_true_iff.
-    - split; apply eq_sym.
-    - split; apply univ_expr_eqb_true_iff.
-  Qed.
-
-
-  Lemma LevelExprSet_for_all_false f u :
-    LevelExprSet.for_all f u = false -> LevelExprSet.exists_ (negb ∘ f) u.
-  Proof.
-    intro H. rewrite LevelExprSetFact.exists_b.
-    rewrite LevelExprSetFact.for_all_b in H.
-    all: try now intros x y [].
-    induction (LevelExprSet.elements u); cbn in *; [discriminate|].
-    apply andb_false_iff in H; apply orb_true_iff; destruct H as [H|H].
-    left; now rewrite H.
-    right; now rewrite IHl.
-  Qed.
-
-  Lemma LevelExprSet_For_all_exprs (P : LevelExpr.t -> Prop) (u : nonEmptyLevelExprSet)
-    : LevelExprSet.For_all P u
-      <-> P (to_nonempty_list u).1 /\ Forall P (to_nonempty_list u).2.
-  Proof.
-    etransitivity.
-    - eapply iff_forall; intro e. eapply imp_iff_compat_r.
-      apply In_to_nonempty_list.
-    - cbn; split.
-      + intro H. split. apply H. now left.
-        apply Forall_forall. intros x H0.  apply H; now right.
-      + intros [H1 H2] e [He|He]. subst e; tas.
-        eapply Forall_forall in H2; tea.
-  Qed.
-
-  Lemma add_comm {le le' e} : add le (add le' e) = add le' (add le e).
-  Proof.
-    apply eq_univ_equal. intros x.
-    rewrite !LevelExprSet.add_spec. firstorder.
-  Qed.
-
-  #[program]
-  Definition univ_union (prems prems' : nonEmptyLevelExprSet) : nonEmptyLevelExprSet :=
-    {| t_set := LevelExprSet.union prems prems' |}.
-  Next Obligation.
-    destruct prems, prems'; cbn.
-    destruct (LevelExprSet.is_empty (LevelExprSet.union _ _)) eqn:ise => //.
-    eapply LevelExprSetFact.is_empty_2 in ise.
-    eapply not_Empty_is_empty in t_ne0, t_ne1.
-    destruct t_ne0. lesets.
-  Qed.
-
-  Lemma univ_union_spec u u' l :
-    LevelExprSet.In l (univ_union u u') <->
-    LevelExprSet.In l u \/ LevelExprSet.In l u'.
-  Proof.
-    destruct u, u'; unfold univ_union; cbn.
-    apply LevelExprSet.union_spec.
-  Qed.
-
-  Lemma univ_union_add_singleton u le : univ_union u (singleton le) = add le u.
-  Proof.
-    apply eq_univ_equal.
-    intros x. rewrite univ_union_spec LevelExprSet.singleton_spec add_spec.
-    intuition auto.
-  Qed.
-
-  Lemma univ_union_comm {u u'} : univ_union u u' = univ_union u' u.
-  Proof.
-    apply eq_univ_equal.
-    intros x. rewrite !univ_union_spec.
-    intuition auto.
-  Qed.
-
-  Lemma univ_union_add_distr {le u u'} : univ_union (add le u) u' = add le (univ_union u u').
-  Proof.
-    apply eq_univ_equal.
-    intros x. rewrite !univ_union_spec !add_spec !univ_union_spec.
-    intuition auto.
-  Qed.
-
-End NonEmptySetFacts.
-Export NonEmptySetFacts.
 
 Lemma diff_eq U V : LevelSet.diff V U =_lset V <-> LevelSet.inter V U =_lset LevelSet.empty.
 Proof. split. lsets. lsets. Qed.
@@ -452,7 +183,7 @@ Lemma levels_exprs_non_W_atoms {W prem} :
   LevelSet.Equal (levels (non_W_atoms W prem)) (LevelSet.diff (levels prem) W).
 Proof.
   intros e. unfold non_W_atoms.
-  rewrite levelexprset_levels_spec LevelSet.diff_spec levelexprset_levels_spec.
+  rewrite levels_spec LevelSet.diff_spec levels_spec.
   firstorder eauto.
   rewrite LevelExprSet.filter_spec in H. now exists x.
   rewrite LevelExprSet.filter_spec in H. destruct H.
@@ -468,8 +199,8 @@ Proof.
   split.
   - intros he.
     intros l hin.
-    eapply levelexprset_levels_spec in hin as [k hin]. lesets.
-  - intros emp l hin. eapply emp. eapply (levelexprset_levels_spec l.1). exists l.2.
+    eapply levels_spec in hin as [k hin]. lesets.
+  - intros emp l hin. eapply emp. eapply (levels_spec l.1). exists l.2.
     now destruct l.
 Qed.
 
